\documentclass[]{article}
\usepackage[margin=1.25in]{geometry}
\usepackage{amsmath,amsthm}
\usepackage{amsfonts}
\usepackage{graphicx,tikz}

%opening
\title{Common Power Series}
\author{Vincent La}

\begin{document}

\maketitle

\section{Formulas}
\subsection{MacLaurin Series}
\[\begin{aligned}
f(z) &= \sum^{n}_{n=0} a_n z^n & \text{where } a_n = \frac{f^{(n)}(0)}{n!}
\end{aligned}\]

\section{Exponential Function}
\subsection{MacLaurin Series}
The MacLaurin series for $e^z$ is 
\[e^z  = \sum^{\infty}_{n=0} \frac{z^n}{n!} \]
which converges for $|z| < \infty$.

\subsubsection{Formula for Series}
\begin{proof}
	Because $\frac{d}{dz} e^z = e^z$, $f^{(n)}(z) = e^z$ which implies $f^{(n)}(0) = 1$. 
	
	\bigskip
	
	Continuing, this means
	\[a_n = \frac{1}{n!} \]
	
	so plugging into the general MacLaurin Series formula we get
	\[e^z = \sum^{\infty}_{n=0} \frac{z^n}{n!}\]
\end{proof}
	
\subsubsection{Convergence}
\begin{proof}
	Let $z \in \mathbb{C}$ be arbitrary and recall that
	\[\sum^{\infty}_{n=0} \frac{z^n}{n!} = \lim_{n \rightarrow \infty} S_n \]
	
	Expanding the partial sum on the RHS, we get
	\[
	\lim_{n \rightarrow \infty} S_n
	= \lim_{n \rightarrow \infty} \frac{z^0}{0!} + \frac{z^1}{1!} + \frac{z^2}{2!} +
	... + \frac{z^n}{n!}
	\]
	
	Now, let us show that the limit of the $n^{th}$ term (denoted $a_n$) is zero.
	\[
	\lim_{n \rightarrow \infty} a_n
	= \lim_{n \rightarrow \infty} \frac{z^n}{n!}
	= \lim_{n \rightarrow \infty} \frac{z \cdot z \cdot z \cdot z \cdot ... \cdot z \cdot ... \cdot z}{0 \cdot 1 \cdot 2 \cdot ... \cdot z \cdot ... \cdot n}
	\]
	
	Because $\lim_{n \rightarrow \infty} \frac{z}{n} = 0$, by the limit of products
	\[\lim_{n \rightarrow \infty} a_n = 0\]
	
	So, as $n \rightarrow \infty$, the $n^{th}$ term of the partial sum is 0, while all the preceding terms are finite. Therefore, $\sum^{\infty}_{n=0} \frac{z^n}{n!}$ converges for all $z$.
\end{proof}

\end{document}
